lib/Multiset_More.thy
@@ -101,7 +101,7 @@ qed
 lemma diff_size_le_size_Diff: "size (\<Sigma>:: _ multiset) - size \<Sigma>' \<le> size (\<Sigma> - \<Sigma>')"
 proof-
   have "size \<Sigma> - size \<Sigma>' \<le> size \<Sigma> - size (\<Sigma> \<inter># \<Sigma>')"
-    using size_mset_mono diff_le_mono2 subset_mset.inf_le2 by blast
+    using size_mset_mono diff_le_mono2 subset_mset.inf_le2 by metis
   also have "\<dots> = size(\<Sigma>-\<Sigma>')" by(simp add: size_Diff_subset_Int)
   finally show ?thesis .
 qed
