Makefile
@@ -37,7 +37,7 @@ all: Weidenbach_Book Bachmair_Ganzinger Unordered_Resolution
 
 # build the documentation and the files
 current: Bachmair_Ganzinger Unordered_Resolution
-	$(RUN_ISABELLE) build -o browser_info -o "document=pdf" -o "document_variants=document:outline=/proof,/ML;userguide" -v -d Weidenbach_Book Full
+	$(RUN_ISABELLE) build -d '$$AFP' -o browser_info -o "document=pdf" -o "document_variants=document:outline=/proof,/ML;userguide" -v -d Weidenbach_Book Full
 
 # need to be in the IJCAR branch
 conference:
